Putting in some changes so I can update to new vale

src/crypto/loopunroll/seq.tobeproved.dfy
@@ -15,18 +15,104 @@ import opened x64_vale_i
 import opened dafny_wrappers_i
 import opened addrlogic
 
-lemma lemma_OnlyWritesAddrs64_Preserves_ValidSrcAlAddrs64
-         (mem0 : Heaplets, mem1: Heaplets, id:heaplet_id, addr : uint64, count_items : nat, 
+/*
+predicate OnlyWritesAddrs64'(old_mem : Heaplets, mem : Heaplets, id:heaplet_id, ar : Addrs64, taint : taint)
+{
+  ValidAddrs64(ar) && 
+  ValidDstUnAddrs64(old_mem, id, ar) && 
+  // mem[id] is still a Healplet64
+  id in mem && mem[id].Heaplet64? && 
+  // I don't delete any of my addresess in id.
+  (forall naddr : int :: naddr in old_mem[id].mem64 ==> naddr in mem[id].mem64) && 
+
+  // I only adjusted addresses in range.
+  (forall naddr : int ::
+    ((naddr < ar.addr || naddr > ar.addr + (ar.count - 1) * 8)  && 
+     (naddr in old_mem[id].mem64 && naddr in mem[id].mem64)) ==>
+    mem[id].mem64[naddr] == old_mem[id].mem64[naddr] &&
+    mem[id].mem64[naddr].t == taint)
+}
+
+lemma lemma_OnlyWritesAddrs64(old_mem : Heaplets, mem : Heaplets, id:heaplet_id, ar : Addrs64, taint : taint)
+  requires OnlyWritesAddrs64(old_mem, mem, id, ar);
+  ensures id in mem;
+  ensures mem[id].Heaplet64?;
+  ensures forall naddr : int :: naddr in old_mem[id].mem64 ==> naddr in mem[id].mem64;
+{
+}
+*/
+
+
+/*
+lemma lemma_WritesAddr64_OnlyWritesAddrs64_Preserves_ValidSrcAlAddrs64
+         (mem0 : Heaplets, mem1: Heaplets, id:heaplet_id, addr : uint64, 
          items : nat, taint : taint, v : seq<uint64>)
-   requires count_items <= items;
    requires ValidSrcAlAddrs64(mem0, id, addrs64(addr, items), taint);
-   requires WritesAddrs64(mem0, mem1, id, addrs64(addr, count_items), taint, v);
-   requires OnlyWritesAddrs64(mem0, mem1, id, addrs64(addr, count_items));
+   requires WritesAddrs64(mem0, mem1, id, addrs64(addr, items), taint, v);
+   requires OnlyWritesAddrs64(mem0, mem1, id, addrs64(addr, items));
    ensures  ValidSrcAlAddrs64(mem1, id, addrs64(addr, items), taint);
 {
 }
 
-lemma lemma_OnlyWritesAddrs64_Preserves_ValidSrcAlAddrs64'
+
+lemma lemma_WritesAddr64_OnlyWritesAddrs64_Preserves_ValidSrcAlAddr64'
+         (mem0 : Heaplets, mem1: Heaplets, id:heaplet_id, 
+          base : uint64, ptr : uint64,
+          items : nat,  more_items : nat, 
+          taint : taint, v : seq<uint64>)
+   requires |v| == items + more_items;
+   requires ptr == base + items * 8;          
+   requires ValidSrcAlAddrs64(mem0, id, addrs64(base, items + more_items), taint);
+   requires WritesAddrs64(mem0, mem1, id, addrs64(ptr, more_items), taint, v[items..(items+more_items)]);
+   requires OnlyWritesAddrs64(mem0, mem1, id, addrs64(ptr, more_items));
+   ensures (forall i : nat :: 0 <= i < items + more_items ==>
+              ValidSrcAlAddr64(mem1, id, addroff64(base, i), taint));
+{
+  lemma_ValidSrcAlAddrs64(mem0, id, addrs64(base, items + more_items), taint);
+  if (items > 0) {
+    assert ValidSrcAlAddr64(mem1, id, addroff64(base, 1), taint);
+  } else {
+  }
+}
+*/
+
+/*
+lemma  lemma_WritesAddr64_OnlyWritesAddrs64_Preserves_ValidSrcAlAddrs64'
+         (mem0 : Heaplets, mem1: Heaplets, id:heaplet_id, 
+          base : uint64, ptr : uint64,
+          items : nat,  more_items : nat, 
+          taint : taint, v : seq<uint64>)
+   requires items > 0;
+   requires |v| == items + more_items;
+   requires ptr == base + items * 8;          
+
+   requires ValidSrcAlAddrs64(mem0, id, addrs64(base, items + more_items), taint);
+   requires WritesAddrs64(mem0, mem1, id, addrs64(ptr, more_items), taint, v[items..(items+more_items)]);
+   requires OnlyWritesAddrs64(mem0, mem1, id, addrs64(ptr, more_items));
+   ensures ValidSrcAlAddr64(mem1, id, addroff64(base, 1), taint);
+{
+}
+*/
+
+/*
+lemma  lemma_WritesAddr64_OnlyWritesAddrs64_Preserves_ValidSrcAlAddrs64'
+         (mem0 : Heaplets, mem1: Heaplets, id:heaplet_id, 
+          base : uint64, ptr : uint64,
+          items : nat,  more_items : nat, 
+          taint : taint, v : seq<uint64>)
+   requires |v| == items + more_items;
+   requires ptr == base + items * 8;          
+   requires ValidSrcAlAddrs64(mem0, id, addrs64(base, items + more_items), taint);
+   requires WritesAddrs64(mem0, mem1, id, addrs64(ptr, more_items), taint, v[items..(items+more_items)]);
+   requires OnlyWritesAddrs64(mem0, mem1, id, addrs64(ptr, more_items));
+   ensures  ValidSrcAlAddrs64(mem1, id, addrs64(base, items + more_items), taint);
+{
+  lemma_ValidSrcAlAddrs64_Tails(mem0, id, addrs64(base, items + more_items), taint);
+}
+*/
+
+/*
+lemma {:timeLimitMultiplier 3} lemma_OnlyWritesAddrs64_Preserves_ValidSrcAlAddrs64'
          (mem0 : Heaplets, mem1: Heaplets, mem2: Heaplets, id:heaplet_id,
           base : uint64, ptr : uint64, 
           items : nat, more_items : nat, 
@@ -38,46 +124,110 @@ lemma lemma_OnlyWritesAddrs64_Preserves_ValidSrcAlAddrs64'
     requires ValidSrcAlAddrs64(mem1, id, addrs64(base, items + more_items), taint);
     
     requires WritesAddrs64(mem0, mem1, id, addrs64(base, items), taint, v[..items]);
-    requires OnlyWritesAddrs64(mem0, mem1, id, addrs64(base, items));
+    requires OnlyWritesAddrs64'(mem0, mem1, id, addrs64(base, items), taint);
 
     requires WritesAddrs64(mem1, mem2, id, addrs64(ptr, more_items), taint, v[items..(items+more_items)]);
-    requires OnlyWritesAddrs64(mem1, mem2, id, addrs64(ptr, more_items));
+    requires OnlyWritesAddrs64'(mem1, mem2, id, addrs64(ptr, more_items), taint);
  
     ensures  ValidSrcAlAddrs64(mem2, id, addrs64(base, items + more_items), taint);
 {
   lemma_subsequence_ext(items, more_items, v);
   lemma_ValidSrcAlAddrs64(mem0, id, addrs64(base, items + more_items), taint);
   lemma_ValidSrcAlAddrs64(mem1, id, addrs64(base, items + more_items), taint);
-  assume ValidSrcAlAddrs64(mem2, id, addrs64(base, items + more_items), taint);
+  lemma_WritesAddr64_OnlyWritesAddrs64_Preserves_ValidSrcAlAddrs64'
+         (mem1, mem2, id, base, ptr, items, more_items, taint, v);
+//  assume ValidSrcAlAddrs64(mem2, id, addrs64(base, items + more_items), taint);
+}
+*/
+
+predicate ValidSrcAlAddrs64'(mem:Heaplets, id:heaplet_id, ar : Addrs64, taint:taint)
+{
+  ValidAddrs64(ar) &&
+  id in mem &&
+  mem[id].Heaplet64? &&
+  EvalAddrOff64(addroff64(ar.addr, 0)) % 8 == 0 && 
+  (forall i : nat :: 0 <= i < ar.count ==> ValidAddrOff64(addroff64(ar.addr, i))) &&
+  (forall i : nat :: 0 <= i < ar.count ==> EvalAddrOff64(addroff64(ar.addr, i)) in mem[id].mem64) &&
+  (forall i : nat :: 0 <= i < ar.count ==> ValidSrcAlAddr64(mem, id, addroff64(ar.addr, i), taint))
 }
 
-lemma {:timeLimitMultiplier 3} lemma_OnlyWrites_Range_Range_Ext
-         (mem0 : Heaplets, mem1: Heaplets, mem2: Heaplets, id : heaplet_id, 
-         base : uint64, ptr : uint64, items : nat, more_items : nat, taint : taint)
-    requires ptr == base + items * 8;
-    requires ValidSrcAlAddrs64(mem0, id, addrs64(base, items + more_items), taint);
-    requires ValidSrcAlAddrs64(mem1, id, addrs64(base, items + more_items), taint);
-    requires ValidSrcAlAddrs64(mem2, id, addrs64(base, items + more_items), taint);
+predicate OnlyWritesAddrs64'(old_mem : Heaplets, mem : Heaplets, id:heaplet_id, ar : Addrs64)
+{  
+  ValidAddrs64(ar) && 
+  ValidDstUnAddrs64(old_mem, id, ar) && 
+  // mem[id] is still a Healplet64
+  id in mem && mem[id].Heaplet64? && 
+  // I don't delete any of my addresess in id.
+  (forall naddr : int :: naddr in old_mem[id].mem64 ==> naddr in mem[id].mem64) && 
 
-    requires OnlyWritesAddrs64(mem0, mem1, id, addrs64(base, items));
+  // I only adjusted values in range.
+  (forall naddr : int ::
+    ((naddr < ar.addr || naddr > ar.addr + (ar.count - 1) * 8)  && 
+     (naddr in old_mem[id].mem64 && naddr in mem[id].mem64)) ==>
+    mem[id].mem64[naddr].v == old_mem[id].mem64[naddr].v) &&
+
+  // I have only adjusted taint in range.
+  (forall naddr : int ::
+    ((naddr < ar.addr || naddr > ar.addr + (ar.count - 1) * 8)  && 
+     (naddr in old_mem[id].mem64 && naddr in mem[id].mem64)) ==>
+    mem[id].mem64[naddr].t == old_mem[id].mem64[naddr].t)
+}
+
+lemma isolate_taint(mem1: Heaplets, mem2: Heaplets, 
+              id:heaplet_id, base : uint64, ptr : uint64, 
+             items: nat, count_items : nat, more_items : nat, taint : taint, v : seq<uint64>)
+    requires items > count_items + more_items;
+    requires |v| == count_items + more_items;
+    requires ptr == base + count_items * 8;
+
+    requires ValidSrcAlAddrs64(mem1, id, addrs64(base, items), taint);
+    requires WritesAddrs64(mem1, mem2, id, addrs64(ptr, more_items), taint, v[count_items..(count_items+more_items)]);
     requires OnlyWritesAddrs64(mem1, mem2, id, addrs64(ptr, more_items));
 
-    ensures  OnlyWritesAddrs64(mem0, mem2, id, addrs64(base, items + more_items));
-{
-  lemma_ValidSrcAlAddrs64(mem0, id, addrs64(base, items + more_items), taint);
-  lemma_ValidSrcAlAddrs64(mem1, id, addrs64(base, items + more_items), taint);
-  lemma_ValidSrcAlAddrs64(mem2, id, addrs64(base, items + more_items), taint);
-}    
+    ensures forall i : nat :: 0 <= i < more_items ==> 
+       mem2[id].mem64[EvalAddrOff64(addroff64(ptr,i))].t == taint;
 
-lemma {:timeLimitMultiplier 3} lemma_Writes_OnlyWrites_Range_Range_Ext
+    ensures forall i : nat :: 0 <= i < more_items ==> 
+       mem2[id].mem64[EvalAddrOff64(addroff64(base + count_items * 8,i))].t == taint;
+
+    ensures forall i : nat :: 0 <= i < items ==> 
+      mem2[id].mem64[EvalAddrOff64(addroff64(base,i))].t == taint;
+{
+  assert forall i : nat :: 0 <= i < items ==>
+   mem1[id].mem64[EvalAddrOff64(addroff64(base,i))].t == taint;
+}
+
+/*
+lemma isolate_ValidSrAlAddrs64(mem1: Heaplets, mem2: Heaplets, 
+              id:heaplet_id, base : uint64, ptr : uint64, 
+             items: nat, count_items : nat, more_items : nat, taint : taint, v : seq<uint64>)
+    requires items > count_items + more_items;
+    requires |v| == count_items + more_items;
+    requires ptr == base + count_items * 8;
+
+    requires ValidSrcAlAddrs64'(mem1, id, addrs64(base, items), taint);
+    requires WritesAddrs64(mem1, mem2, id, addrs64(ptr, more_items), taint, v[count_items..(count_items+more_items)]);
+    requires OnlyWritesAddrs64(mem1, mem2, id, addrs64(ptr, more_items));
+
+    ensures ValidSrcAlAddrs64'(mem2, id, addrs64(base, items), taint);
+{
+  forall i : nat | 0 <= i < items
+    ensures ValidSrcAlAddr64(mem2, id, addroff64(base, i), taint);
+  {
+  }
+}
+*/
+
+/*
+lemma lemma_Writes_OnlyWrites_Range_Range_Ext
          (mem0 : Heaplets, mem1: Heaplets, mem2: Heaplets, 
           id:heaplet_id, base : uint64, ptr : uint64, 
           items: nat, count_items : nat, more_items : nat, taint : taint, v : seq<uint64>)
     requires items > count_items + more_items;
     requires |v| == count_items + more_items;
     requires ptr == base + count_items * 8;
-    requires ValidSrcAlAddrs64(mem0, id, addrs64(base, items), taint);
-    requires ValidSrcAlAddrs64(mem1, id, addrs64(base, items), taint);
+    requires ValidSrcAlAddrs64'(mem0, id, addrs64(base, items), taint);
+    requires ValidSrcAlAddrs64'(mem1, id, addrs64(base, items), taint);
     
     requires WritesAddrs64(mem0, mem1, id, addrs64(base, count_items), taint, v[..count_items]);
     requires OnlyWritesAddrs64(mem0, mem1, id, addrs64(base, count_items));
@@ -85,17 +235,21 @@ lemma {:timeLimitMultiplier 3} lemma_Writes_OnlyWrites_Range_Range_Ext
     requires WritesAddrs64(mem1, mem2, id, addrs64(ptr, more_items), taint, v[count_items..(count_items+more_items)]);
     requires OnlyWritesAddrs64(mem1, mem2, id, addrs64(ptr, more_items));
 
-    ensures ValidSrcAlAddrs64(mem2, id, addrs64(base, items), taint);
+    ensures ValidSrcAlAddrs64'(mem2, id, addrs64(base, items), taint);
+    //  (forall i : nat :: 0 <= i < ar.count ==> ValidSrcAlAddr64(mem2, id, addroff64(ar.addr, i), taint))
     ensures WritesAddrs64(mem0, mem2, id, addrs64(base, count_items + more_items), taint, v);
+    //   ValidSrcAlAddrs64(mem2, id, ar, taint)
+    // (forall i : nat :: 0 <= i < ar.count ==> ValidSrcAlAddr64(mem2, id, addroff64(ar.addr, i), taint))
     ensures OnlyWritesAddrs64(mem0, mem2, id, addrs64(base, count_items + more_items));
 { 
   lemma_subsequence_ext(count_items, more_items, v);
   lemma_ValidSrcAlAddrs64(mem0, id, addrs64(base, count_items + more_items), taint);
   lemma_ValidSrcAlAddrs64(mem1, id, addrs64(base, count_items + more_items), taint);
-  lemma_OnlyWritesAddrs64_Preserves_ValidSrcAlAddrs64'
-         (mem0, mem1, mem2, id, base, ptr, count_items, more_items, taint, v);
-  lemma_OnlyWrites_Range_Range_Ext(mem0, mem1, mem2, id, base, ptr, count_items, more_items, taint);
+//  lemma_OnlyWritesAddrs64_Preserves_ValidSrcAlAddrs64'
+//         (mem0, mem1, mem2, id, base, ptr, count_items, more_items, taint, v);
+//  lemma_OnlyWrites_Range_Range_Ext(mem0, mem1, mem2, id, base, ptr, count_items, more_items, taint);
 }
+*/
 
 }
 
